variant of compactness

theories/WKL.v
@@ -102,24 +102,23 @@ Definition compactness (C : forall Sigma D, @interp Sigma D -> Prop) :=
   forall {HdF : eq_dec Funcs} {HdP : eq_dec Preds},
   forall {HeF : enumT Funcs} {HeP : enumT Preds},
   forall T (T_closed : closed_T T),
-  (forall Gamma, Gamma ⊏ T -> exists D (I : interp D) rho, C Sigma D I /\ forall phi, phi el Gamma -> rho ⊨ phi)
+  (forall Gamma, Gamma ⊏ T -> exists D (I : interp D) rho, SM I /\ forall phi, phi el Gamma -> rho ⊨ phi)
   -> exists D (I : interp D) rho, C Sigma D I /\ forall phi, phi ∈ T -> rho ⊨ phi.
 
 Lemma modex_compact (C : forall Sigma D, @interp Sigma D -> Prop) :
-  (forall Sigma D I, C Sigma D I -> @SM Sigma D I) -> model_existence' C -> compactness C.
+  model_existence' C -> compactness C.
 Proof.
-  intros HC HM Sigma HdF HdP HeF HeP T T_closed H.
+  intros HM Sigma HdF HdP HeF HeP T T_closed H.
   apply HM in T_closed as (D & I & rho & _ & _ & HI); trivial.
   + intros [Gamma [H1 H2]]. apply H in H1 as (D & I & rho & H3 & H4).
-    apply HC in H3. apply Soundness' in H2.
-    apply H3. now apply (H2 D I H3 rho).
+    apply Soundness' in H2. apply H3. now apply (H2 D I H3 rho).
   + now exists D, I, rho.
 Qed.
 
 Lemma compact_standard :
   compactness (@SM).
 Proof.
-  apply modex_compact; try tauto. apply modex_standard.
+  apply modex_compact. apply modex_standard.
 Qed.
 
 Definition DM `{Signature} D (I : interp D) := classical I /\ standard_bot I /\ GenTarski.decidable I.
